VerifiedFilter/Regex/Num.lean
@@ -5,7 +5,8 @@ import VerifiedFilter.Regex.Regex
 namespace Regex
 
 @[reducible, simp]
-def symbols: (r: Regex σ) → Nat
+def symbols (r: Regex σ): Nat :=
+  match r with
   | emptyset => 0 | emptystr => 0 | symbol _ => 1 | star r1 => symbols r1
   | or r1 r2 => symbols r1 + symbols r2 | concat r1 r2 => symbols r1 + symbols r2
   | interleave r1 r2 => symbols r1 + symbols r2
